JaIrisProof.v
@@ -1,0 +1,111 @@
+Require Import String.
+Require Import NPeano.
+Require Import PeanoNat.
+Require Import Coq.Strings.Ascii.
+Require FMapWeakList.
+Require Export Coq.Structures.OrderedTypeEx.
+Require Import Lists.List.
+Import ListNotations.
+Require Import JaSyntax.
+Require Import JaTypes.
+Require Import JaProgram.
+Require Import JaEnvs.
+Require Import Jafun.
+Require Import JaSubtype.
+Require Import Bool.
+Require Import JaIrisPermutation.
+Require Import JaIrisCommon.
+Require Import JaIris.
+Require Import Classical_Prop.
+
+Require Export FMapAVL.
+Require Export Coq.Structures.OrderedTypeEx.
+Require Import FMapFacts.
+
+Module StrMap := JaIrisCommon.StrMap.
+
+Definition FreeVarsInTermAreInGammaOrX e (gamma : JFITypeEnv) x :=
+  forall y, VarFreeInTerm y e -> (y = x \/ StrMap.In y gamma).
+
+Lemma FreeVarsInTrue : forall gamma,
+  FreeVarsInTermAreInGamma JFITrue gamma <-> True.
+Proof.
+Admitted.
+
+Lemma FreeVarsInFalse : forall gamma,
+  FreeVarsInTermAreInGamma JFIFalse gamma <-> True.
+Proof.
+Admitted.
+
+Lemma FreeVarsInAnd : forall gamma p q,
+  FreeVarsInTermAreInGamma (JFIAnd p q) gamma <->
+  (FreeVarsInTermAreInGamma p gamma /\ FreeVarsInTermAreInGamma q gamma).
+Proof.
+Admitted.
+
+Lemma FreeVarsInOr : forall gamma p q,
+  FreeVarsInTermAreInGamma (JFIOr p q) gamma <->
+  (FreeVarsInTermAreInGamma p gamma /\ FreeVarsInTermAreInGamma q gamma).
+Proof.
+Admitted.
+
+Lemma FreeVarsInImplies : forall gamma p q,
+  FreeVarsInTermAreInGamma (JFIImplies p q) gamma <->
+  (FreeVarsInTermAreInGamma p gamma /\ FreeVarsInTermAreInGamma q gamma).
+Proof.
+Admitted.
+
+Lemma FreeVarsInHoare : forall gamma p e ex v q,
+  FreeVarsInTermAreInGamma (JFIHoare p e ex v q) gamma <->
+  (FreeVarsInTermAreInGamma p gamma /\ FreeVarsInExprAreInGamma e gamma /\
+    (FreeVarsInTermAreInGammaOrX q gamma v)).
+Proof.
+Admitted.
+
+Lemma FreeVarsInEq : forall gamma v1 v2,
+  FreeVarsInTermAreInGamma (JFIEq v1 v2) gamma <->
+  (FreeVarsInValAreInGamma v1 gamma /\ FreeVarsInValAreInGamma v2 gamma).
+Proof.
+Admitted.
+Hint Resolve FreeVarsInEq : free_vars_in_gamma.
+
+Lemma FreeVarsInFieldEq : forall gamma o f v,
+  FreeVarsInTermAreInGamma (JFIFieldEq o f v) gamma <->
+  (FreeVarsInValAreInGamma o gamma /\ FreeVarsInValAreInGamma v gamma).
+Proof.
+Admitted.
+Hint Resolve FreeVarsInEq : free_vars_in_gamma.
+
+Lemma FreeVarsInSep : forall gamma p q,
+  FreeVarsInTermAreInGamma (JFISep p q) gamma <->
+  (FreeVarsInTermAreInGamma p gamma /\ FreeVarsInTermAreInGamma q gamma).
+Proof.
+Admitted.
+
+Lemma FreeVarsInWand : forall gamma p q,
+  FreeVarsInTermAreInGamma (JFIWand p q) gamma <->
+  (FreeVarsInTermAreInGamma p gamma /\ FreeVarsInTermAreInGamma q gamma).
+Proof.
+Admitted.
+
+
+Ltac try_solve_free_vars :=
+  try rewrite !FreeVarsInAnd in *;
+  try rewrite !FreeVarsInOr in *;
+  try rewrite !FreeVarsInImplies in *;
+  try rewrite !FreeVarsInEq in *;
+  try rewrite !FreeVarsInFieldEq in *;
+  try rewrite !FreeVarsInSep in *;
+  try rewrite !FreeVarsInWand in *;
+  try rewrite !FreeVarsInTrue in *;
+  try rewrite !FreeVarsInFalse in *;
+  try easy.
+
+Lemma FreeVarsAreInGamma : forall decls gamma p q,
+  JFIProves decls gamma p q ->
+  (FreeVarsInTermAreInGamma p gamma /\ FreeVarsInTermAreInGamma q gamma).
+Proof.
+  intros decls gamma p q proof.
+  induction proof; try_solve_free_vars.
+  (* TODO Hoare *)
+Admitted.
